ironfleet/src/Dafny/Distributed/Protocol/RSL/FailureProof/Phase2_PostFail/GenericLemmas.i.dfy
@@ -1,0 +1,259 @@
+include "Phase2Proof.i.dfy"
+
+module RslPhase2Proof_PostFail_Generic {
+import opened RslPhase2Proof_PostFail_i
+
+/* WARNING: this file a timeout of 60s to verify */
+
+
+/* There can be no 2b messages in the system before there are 2a's */
+lemma {:timeLimitMultiplier 2} lemma_NoNew2bBefore2aSent(ts:TimestampedRslState, ts':TimestampedRslState, opn:OperationNumber, idx:int, tios:seq<TimestampedLIoOp<NodeIdentity, RslMessage>>) 
+    requires P2Assumption(ts, opn) && RslConsistency(ts)
+    requires P2Assumption(ts', opn) && RslConsistency(ts')
+    requires PacketsBallotInvariant(ts) && PacketsBallotInvariant(ts')
+    requires TimestampedRslNext(ts, ts')
+    requires !TimestampedRslNextEnvironment(ts, ts')
+    requires TimestampedRslNextOneReplica(ts, ts', idx, tios)
+    requires Before_2a_Sent_Invariant(ts, opn)
+    ensures !exists pkt :: pkt in ts'.t_environment.sentPackets && IsNew2bPacket(pkt, opn)
+{
+    var ls, ls' := ts.t_replicas[idx], ts'.t_replicas[idx];
+    var nextActionIndex := ls.v.nextActionIndex;
+    forall p | p in ts'.t_environment.sentPackets 
+    ensures !IsNew2bPacket(p, opn) {
+        if IsNew2bPacket(p, opn) {
+            assert p !in ts.t_environment.sentPackets;
+            if nextActionIndex == 0 {
+                assert !IsNew2aPacket(tios[0].r, opn);
+                forall io | io in tios && io.LIoOpSend? 
+                ensures !IsNew2bPacket(io.s, opn) {}
+                assert false;
+            } else {
+                assert forall io | io in tios && io.LIoOpSend? :: !io.s.msg.v.RslMessage_2b?;
+                assert false;
+            }
+        }
+    }
+}
+
+
+// /* There can be no 1b messages in the system before there are 1a's */
+// lemma lemma_No1bBefore1aSent(ts:TimestampedRslState, ts':TimestampedRslState, opn:OperationNumber, idx:int, tios:seq<TimestampedLIoOp<NodeIdentity, RslMessage>>) 
+//     requires P2Assumption(ts, opn) && RslConsistency(ts)
+//     requires P2Assumption(ts', opn) && RslConsistency(ts')
+//     requires TimestampedRslNext(ts, ts')
+//     requires !TimestampedRslNextEnvironment(ts, ts')
+//     requires TimestampedRslNextOneReplica(ts, ts', idx, tios)
+//     requires AlwaysInvariant(ts, opn)
+//     ensures forall pkt | pkt in ts'.undeliveredPackets :: !pkt.msg.v.RslMessage_1b?
+// {
+//     var ls, ls' := ts.t_replicas[idx], ts'.t_replicas[idx];
+//     var nextActionIndex := ls.v.nextActionIndex;
+//     forall p | p in ts'.undeliveredPackets
+//     ensures !p.msg.v.RslMessage_1b? {
+//         if p.msg.v.RslMessage_1b? {
+//             assert p !in ts.undeliveredPackets;
+//             if nextActionIndex == 0 {
+//                 assert !tios[0].r.msg.v.RslMessage_1a?;
+//                 assert forall io | io in tios && io.LIoOpSend? :: !io.s.msg.v.RslMessage_1b?;
+//                 assert false;
+//             } else {
+//                 assert forall io | io in tios && io.LIoOpSend? :: !io.s.msg.v.RslMessage_1b?;
+//                 assert false;
+//             }
+//         }
+//     }
+// }
+
+
+// /* Non-leader replicas do not send 2a's */
+lemma lemma_NonLeaderDoesNotSend2a(ts:TimestampedRslState, ts':TimestampedRslState, opn:OperationNumber, idx:int, tios:seq<TimestampedLIoOp<NodeIdentity, RslMessage>>) 
+    requires P2Assumption(ts, opn) && RslConsistency(ts)
+    requires P2Assumption(ts', opn) && RslConsistency(ts')
+    requires TimestampedRslNext(ts, ts')
+    requires !TimestampedRslNextEnvironment(ts, ts')
+    requires TimestampedRslNextOneReplica(ts, ts', idx, tios)
+    requires Before_2a_Sent_Invariant(ts, opn) || Before_2b_Sent_Invariant(ts, opn) || After_2b_Sent_Invariant(ts, opn)
+    requires idx != 1
+    ensures forall p | p in ts'.t_environment.sentPackets && p.msg.v.RslMessage_2a? :: p in ts.t_environment.sentPackets
+    ensures forall p | p in ts'.undeliveredPackets && IsNew2aPacket(p, opn) :: p in ts.undeliveredPackets
+{
+    var ls, ls' := ts.t_replicas[idx], ts'.t_replicas[idx];
+    var nextActionIndex := ls.v.nextActionIndex;
+    forall p | p in ts'.t_environment.sentPackets && p.msg.v.RslMessage_2a?
+    ensures p in ts.t_environment.sentPackets {
+        if p !in ts.t_environment.sentPackets {
+            if nextActionIndex == 3 {
+                assert !LProposerCanNominateUsingOperationNumber(ls.v.replica.proposer, ls.v.replica.acceptor.log_truncation_point, ls.v.replica.proposer.next_operation_number_to_propose);
+                assert forall io | io in tios && io.LIoOpSend? :: !io.s.msg.v.RslMessage_2a?;
+                assert false;
+            } else {
+                assert forall io | io in tios && io.LIoOpSend? :: !io.s.msg.v.RslMessage_2a?;
+                assert false;
+            }
+        }
+    }
+    lemma_NonLeaderDoesNotSend2a_Undelivered(ts, ts', opn, idx, tios);
+}
+
+/* Non-leader replicas do not send 2a's */
+lemma lemma_NonLeaderDoesNotSend2a_Undelivered(ts:TimestampedRslState, ts':TimestampedRslState, opn:OperationNumber, idx:int, tios:seq<TimestampedLIoOp<NodeIdentity, RslMessage>>) 
+    requires P2Assumption(ts, opn) && RslConsistency(ts)
+    requires P2Assumption(ts', opn) && RslConsistency(ts')
+    requires TimestampedRslNext(ts, ts')
+    requires !TimestampedRslNextEnvironment(ts, ts')
+    requires TimestampedRslNextOneReplica(ts, ts', idx, tios)
+    requires Before_2a_Sent_Invariant(ts, opn) || Before_2b_Sent_Invariant(ts, opn) || After_2b_Sent_Invariant(ts, opn)
+    requires idx != 1
+    ensures forall p | p in ts'.undeliveredPackets && IsNew2aPacket(p, opn) :: p in ts.undeliveredPackets
+{
+    var ls, ls' := ts.t_replicas[idx], ts'.t_replicas[idx];
+    var nextActionIndex := ls.v.nextActionIndex;
+    forall p | p in ts'.undeliveredPackets && IsNew2aPacket(p, opn)
+    ensures p in ts.undeliveredPackets {
+        if p !in ts.undeliveredPackets {
+            if nextActionIndex == 3 {
+                assert !LProposerCanNominateUsingOperationNumber(ls.v.replica.proposer, ls.v.replica.acceptor.log_truncation_point, ls.v.replica.proposer.next_operation_number_to_propose);
+                assert forall io | io in tios && io.LIoOpSend? :: !io.s.msg.v.RslMessage_2a?;
+                assert false;
+            } else {
+                lemma_No2aSentInNon2aStep(ts, ts', opn, idx, tios);
+                assert forall io | io in tios && io.LIoOpSend? :: !io.s.msg.v.RslMessage_2a?;
+                assert false;
+            }
+        }
+    }
+}
+
+// /* Non-leader replicas do not send replies */
+lemma lemma_NonLeaderDoesNotSendReply(ts:TimestampedRslState, ts':TimestampedRslState, opn:OperationNumber, idx:int, tios:seq<TimestampedLIoOp<NodeIdentity, RslMessage>>) 
+    requires P2Assumption(ts, opn) && RslConsistency(ts)
+    requires P2Assumption(ts', opn) && RslConsistency(ts')
+    requires TimestampedRslNext(ts, ts')
+    requires !TimestampedRslNextEnvironment(ts, ts')
+    requires TimestampedRslNextOneReplica(ts, ts', idx, tios)
+    requires Phase2Invariant(ts, opn)
+    requires idx != 1
+    ensures forall p | p in ts'.t_environment.sentPackets && IsNewReplyPacket(ts, p) :: p in ts.t_environment.sentPackets
+{
+    var ls, ls' := ts.t_replicas[idx], ts'.t_replicas[idx];
+    var nextActionIndex := ls.v.nextActionIndex;
+    forall p | p in ts'.t_environment.sentPackets && IsNewReplyPacket(ts, p)
+    ensures p in ts.t_environment.sentPackets {
+        if p !in ts.t_environment.sentPackets {
+            if nextActionIndex == 6 {
+                assert forall io | io in tios && io.LIoOpSend? :: io.s.src == ts'.constants.config.replica_ids[idx];
+                assert p.src == ts'.constants.config.replica_ids[idx];
+                assert ReplicasDistinct(ts'.constants.config.replica_ids, 1, idx);
+                assert false;
+            } else {
+                assert forall io | io in tios && io.LIoOpSend? :: !io.s.msg.v.RslMessage_2a?;
+                assert false;
+            }
+        }
+    }
+}
+
+// /* Non-leader replicas do not send replies */
+// lemma lemma_NonLeaderDoesNotSendReply_Undelivered(ts:TimestampedRslState, ts':TimestampedRslState, opn:OperationNumber, idx:int, tios:seq<TimestampedLIoOp<NodeIdentity, RslMessage>>) 
+//     requires P2Assumption(ts, opn) && RslConsistency(ts)
+//     requires P2Assumption(ts', opn) && RslConsistency(ts')
+//     // requires PacketsBallotInvariant(ts) && PacketsBallotInvariant(ts')
+//     requires TimestampedRslNext(ts, ts')
+//     requires !TimestampedRslNextEnvironment(ts, ts')
+//     requires TimestampedRslNextOneReplica(ts, ts', idx, tios)
+//     requires Phase2Invariant(ts, opn)
+//     requires idx != 0
+//     ensures forall p | p in ts'.undeliveredPackets && IsNewReplyPacket(ts, p) :: p in ts.undeliveredPackets
+// {
+//     var ls, ls' := ts.t_replicas[idx], ts'.t_replicas[idx];
+//     var nextActionIndex := ls.v.nextActionIndex;
+//     forall p | p in ts'.undeliveredPackets && IsNewReplyPacket(ts, p)
+//     ensures p in ts.undeliveredPackets {
+//         if p !in ts.undeliveredPackets {
+//             if nextActionIndex == 6 {
+//                 assert forall io | io in tios && io.LIoOpSend? :: io.s.src == ts'.constants.config.replica_ids[idx];
+//                 assert p.src == ts'.constants.config.replica_ids[idx];
+//                 assert ReplicasDistinct(ts'.constants.config.replica_ids, 0, idx);
+//                 assert false;
+//             } else {
+//                 assert forall io | io in tios && io.LIoOpSend? :: !io.s.msg.v.RslMessage_2a?;
+//                 assert false;
+//             }
+//         }
+//     }
+// }
+
+
+// /* There can be no 2b messages sent in a Non-Receive step  */
+lemma lemma_No2bSentInNonReceiveStep(ts:TimestampedRslState, ts':TimestampedRslState, opn:OperationNumber, idx:int, tios:seq<TimestampedLIoOp<NodeIdentity, RslMessage>>) 
+    requires P2Assumption(ts, opn) && RslConsistency(ts)
+    requires P2Assumption(ts', opn) && RslConsistency(ts')
+    requires TimestampedRslNext(ts, ts')
+    requires !TimestampedRslNextEnvironment(ts, ts')
+    requires TimestampedRslNextOneReplica(ts, ts', idx, tios)
+    requires Phase2Invariant(ts, opn)
+    requires ts.t_replicas[idx].v.nextActionIndex != 0
+    ensures forall pkt | pkt in ts'.t_environment.sentPackets && pkt.msg.v.RslMessage_2b? :: pkt in ts.t_environment.sentPackets
+{
+    var ls, ls' := ts.t_replicas[idx], ts'.t_replicas[idx];
+    var nextActionIndex := ls.v.nextActionIndex;
+    forall pkt | pkt in ts'.t_environment.sentPackets && pkt.msg.v.RslMessage_2b?
+    ensures pkt in ts.t_environment.sentPackets 
+    {
+        if pkt !in ts.t_environment.sentPackets {
+            var ios := UntagLIoOpSeq(tios);
+            var sent_packets := ExtractSentPacketsFromIos(ios);
+            assert LReplicaNoReceiveNext(ls.v.replica, nextActionIndex, ls'.v.replica, ios);
+            assert forall p | p in sent_packets :: !p.msg.RslMessage_2b?;
+            forall io | io in tios && io.LIoOpSend?
+            ensures !io.s.msg.v.RslMessage_2b? {}
+            assert false;
+        }
+    }
+}
+
+/* There can be no 2a messages sent in a Receive step  */
+lemma {:timeLimitMultiplier 2} lemma_No2aSentInNon2aStep(ts:TimestampedRslState, ts':TimestampedRslState, opn:OperationNumber, idx:int, tios:seq<TimestampedLIoOp<NodeIdentity, RslMessage>>) 
+    requires P2Assumption(ts, opn) && RslConsistency(ts)
+    requires P2Assumption(ts', opn) && RslConsistency(ts')
+    requires TimestampedRslNext(ts, ts')
+    requires !TimestampedRslNextEnvironment(ts, ts')
+    requires TimestampedRslNextOneReplica(ts, ts', idx, tios)
+    requires Phase2Invariant(ts, opn)
+    requires ts.t_replicas[idx].v.nextActionIndex != 3
+    ensures forall pkt | pkt in ts'.t_environment.sentPackets && pkt.msg.v.RslMessage_2a? :: pkt in ts.t_environment.sentPackets
+    ensures forall p | p in ts'.undeliveredPackets && IsNew2aPacket(p, opn) :: p in ts.undeliveredPackets
+{
+    var ls, ls' := ts.t_replicas[idx], ts'.t_replicas[idx];
+    var nextActionIndex := ls.v.nextActionIndex;
+    forall p | p in ts'.undeliveredPackets && IsNew2aPacket(p, opn)
+    ensures p in ts.undeliveredPackets {
+        if p !in ts.undeliveredPackets {
+            if nextActionIndex == 3 {
+                assert false;
+            } else {
+                forall io | io in tios && io.LIoOpSend?
+                ensures !io.s.msg.v.RslMessage_2a? {}
+                assert false;
+            }
+        }
+    }
+    forall io | io in tios && io.LIoOpSend?
+    ensures !io.s.msg.v.RslMessage_2a? {}
+}
+
+
+// /* There can be no Reply messages sent in a Non-Execution step  */
+lemma lemma_NoRepliesSentInNonExecutionStep(ts:TimestampedRslState, ts':TimestampedRslState, opn:OperationNumber, idx:int, tios:seq<TimestampedLIoOp<NodeIdentity, RslMessage>>) 
+    requires P2Assumption(ts, opn) && RslConsistency(ts)
+    requires P2Assumption(ts', opn) && RslConsistency(ts')
+    requires TimestampedRslNext(ts, ts')
+    requires !TimestampedRslNextEnvironment(ts, ts')
+    requires TimestampedRslNextOneReplica(ts, ts', idx, tios)
+    requires Phase2Invariant(ts, opn)
+    requires ts.t_replicas[idx].v.nextActionIndex != 6
+    ensures forall pkt | pkt in ts'.t_environment.sentPackets && IsNewReplyPacket(ts', pkt) :: pkt in ts.t_environment.sentPackets
+{}
+
+}
