ironfleet/src/Dafny/Distributed/Protocol/RSL/FailureProof/Phase2_PostFail/verify.sh
@@ -1,11 +1,16 @@
 #!/bin/bash -li
 
+echo ""
+echo "Verifying GenericLemmas.i.dfy"
+dafny GenericLemmas.i.dfy | grep -iv "Warning"
+
+echo ""
 echo "Verifying (long) Phase2Proof_helper0.i.dfy"
 dafnylong Phase2Proof_helper0.i.dfy | grep -iv "Warning"
 
 echo ""
-echo "Verifying (long) Phase2Proof_helper1.i.dfy"
-dafnylong Phase2Proof_helper1.i.dfy | grep -iv "Warning"
+echo "Verifying Phase2Proof_helper1.i.dfy"
+dafny Phase2Proof_helper1.i.dfy | grep -iv "Warning"
 
 echo ""
 echo "Verifying (long) Phase2Proof_helper2.i.dfy"
